theories/prob_eff_lang/probblaze/p_composition.v
@@ -1,0 +1,33 @@
+From iris.proofmode Require Import base proofmode classes.
+From iris.base_logic.lib Require Import na_invariants.
+From iris.algebra Require Import agree excl auth frac excl_auth.
+From iris.algebra.lib Require Import dfrac_agree.
+From clutch Require Import stdpp_ext.
+From clutch.prob_eff_lang.probblaze Require Import logic primitive_laws proofmode
+ spec_rules spec_ra class_instances.
+From clutch.prob_eff_lang.probblaze Require Import tactics.
+From clutch.prob_eff_lang.probblaze Require Import sem_types sem_row sem_sig sem_judgement sem_def.
+
+(*Import fingroup.
+
+Import fingroup.fingroup.
+
+Import valgroup_tactics.
+*)
+Section parallel_composition.
+
+  (*Fixpoint list_args_app (f : val) (op_l : list val) : val :=
+    match: op_l with
+    | nil => f
+    | op_x :: op_{xs} => (f op_x)
+    end.*)
+  
+  
+Definition left_composition (f_x f_y : val) : val := λ: "f" "op_x1" "op_x2" "op_y1" "op_y2",
+                                                                                                       f_x (f_y "f" "op_y1" "op_y2") "op_x1" "op_x2".
+
+Definition right_composition (f_x : val) (f_y : val) (op_x1 op_x2 : val) : val :=
+  λ: "f" "op_x1" "op_x2" "op_y1" "op_y2",
+  (left_composition f_y f_x) "f" "op_y1" "op_y2" "op_x1" "op_x2".
+
+End parallel_composition.
